Major progress in proof CIU -> Vrel

src/FrameStack/CIU.v
@@ -157,27 +157,146 @@ Corollary CIU_compat_reverse :
   forall v v' : Val, CIU (`v) (`v') -> CIU (RValSeq [v]) (RValSeq [v']).
 Proof.
   intros. assert (⟨[], `v⟩ -->* RValSeq [v]). {
-    eexists. split; auto. econstructor. constructor. constructor.
+    apply CIU_closed_l in H. destruct_scopes.
+    eexists. split; auto. econstructor. constructor; auto.
+    econstructor.
   }
   assert (⟨[], `v'⟩ -->* RValSeq [v']). {
-    eexists. split; auto. econstructor. constructor. constructor.
+    apply CIU_closed_r in H. destruct_scopes.
+    eexists. split; auto. econstructor. constructor; auto. constructor.
   }
   apply CIU_eval in H0, H1. 2-3: apply H. intuition.
   epose proof (CIU_transitive_closed _ _ _ H H0).
   now epose proof (CIU_transitive_closed _ _ _ H3 H1).
 Qed.
 
+Lemma match_pattern_list_vars :
+  forall l, match_pattern_list (repeat PVar (length l)) l = Some l.
+Proof.
+  induction l; simpl; auto.
+  break_match_goal; congruence.
+Qed.
+
+Lemma match_pattern_list_tuple_vars :
+  forall l, match_pattern_list [PTuple (repeat PVar (length l))] [VTuple l] = Some l.
+Proof.
+  induction l; simpl; auto.
+  break_match_goal; break_match_hyp; try congruence.
+  - inversion Heqo. simpl in IHl.
+    rewrite Heqo0 in IHl. inv IHl. reflexivity.
+  - simpl in IHl. rewrite Heqo0 in IHl. congruence.
+Qed.
+
+Lemma match_pattern_list_map_vars :
+  forall l, match_pattern_list [PMap (repeat (PVar , PVar) (length l))] [VMap l] = Some (flatten_list l).
+Proof.
+  induction l; simpl; auto.
+  break_match_goal; break_match_hyp; try congruence.
+  - destruct a. inv Heqp. simpl in IHl. break_match_hyp. 2: congruence.
+    inv Heqo. inv IHl. reflexivity.
+  - destruct a. inv Heqp. simpl in IHl. break_match_hyp; congruence.
+Qed.
+
+Fixpoint varsFrom n m : list Val :=
+  match m with
+  | O => []
+  | S m' => VVar n :: varsFrom (S n) m'
+  end.
+
 Lemma Erel_Val_compat_closed_reverse :
   forall (v v' : Val), CIU (`v) (`v') -> forall m, Vrel m v v'.
 Proof.
-  induction v; destruct v'; intros; auto; destruct H as [_ [_ H]].
+  valinduction; try destruct v'; intros; auto; destruct H as [Hcl1 [Hcl2 H]].
   1-7: epose proof (H [FCase1 [([PNil], `ttrue, `VNil);([PVar], `ttrue , °inf)]] ltac:(scope_solver) _) as H0;
-       repeat deriv; inv H8; inv H7; simpl in H10; do 2 deriv; simpl in H8; apply inf_diverges in H8; contradiction.
-  1,3-8: epose proof (H [FCase1 [([PLit l], `ttrue, `VNil);([PVar], `ttrue , °inf)]] ltac:(scope_solver) _) as H0; repeat deriv; inv H8; inv H7; simpl in H10; do 2 deriv; simpl in H8; apply inf_diverges in H8; contradiction.
-  2-3,5-9: epose proof (H [FCase1 [([PCons PVar PVar], `ttrue, `VNil);([PVar], `ttrue , °inf)]] ltac:(scope_solver) _) as H0; repeat deriv; inv H8; inv H7; simpl in H10; do 2 deriv; simpl in H8; apply inf_diverges in H8; contradiction.
-  3-5,7-10: epose proof (H [FCase1 [([PTuple (repeat PVar (length l))], `ttrue, `VNil);([PVar], `ttrue , °inf)]] ltac:(scope_solver) _) as H0; repeat deriv; inv H8; inv H7; simpl in H10; do 2 deriv; simpl in H8; apply inf_diverges in H8; contradiction.
-  4-7,9-11: epose proof (H [FCase1 [([PMap (repeat (PVar, PVar) (length l))], `ttrue, `VNil);([PVar], `ttrue , °inf)]] ltac:(scope_solver) _) as H0; repeat deriv; inv H8; inv H7; simpl in H10; do 2 deriv; simpl in H8; apply inf_diverges in H8; contradiction.
-  5: { admit. }
+       repeat deriv; inv H9; inv H8; simpl in H11; do 2 deriv; simpl in H10; apply inf_diverges in H10; contradiction.
+  1,3-8: epose proof (H [FCase1 [([PLit l], `ttrue, `VNil);([PVar], `ttrue , °inf)]] ltac:(scope_solver) _) as H0; repeat deriv; inv H9; inv H8; simpl in H11; do 2 deriv; simpl in H10; apply inf_diverges in H10; contradiction.
+  2-3,5-9: epose proof (H [FCase1 [([PCons PVar PVar], `ttrue, `VNil);([PVar], `ttrue , °inf)]] ltac:(scope_solver) _) as H0; repeat deriv; inv H9; inv H8; simpl in H11; do 2 deriv; simpl in H10; apply inf_diverges in H10; contradiction.
+  3-5,7-10: epose proof (H [FCase1 [([PTuple (repeat PVar (length l))], `ttrue, `VNil);([PVar], `ttrue , °inf)]] ltac:(scope_solver) _) as H0; repeat deriv; inv H9; inv H8; simpl in H11; do 2 deriv; simpl in H10; apply inf_diverges in H10; contradiction.
+  4-7,9-11: epose proof (H [FCase1 [([PMap (repeat (PVar, PVar) (length l))], `ttrue, `VNil);([PVar], `ttrue , °inf)]] ltac:(scope_solver) _) as H0; repeat deriv; inv H9; inv H8; simpl in H11; do 2 deriv; simpl in H10; apply inf_diverges in H10; contradiction.
+  5-12: destruct_scopes; lia.
+  5-12: destruct_scopes; lia.
+  Unshelve. (* evaluation in the omitted proofs *)
+  13-19: now do 10 econstructor.
+  13-19:
+    econstructor; econstructor; auto; econstructor;
+    [simpl; rewrite Lit_eqb_refl; reflexivity|];
+    simpl; econstructor; auto; econstructor;
+    [simpl; rewrite Lit_eqb_refl; reflexivity|]; constructor; auto;
+    constructor; auto.
+  13-19: 
+    destruct_scopes; econstructor; econstructor; auto; econstructor;
+    [reflexivity|]; simpl; econstructor; auto; econstructor;
+    [reflexivity|]; constructor; auto;
+    constructor; auto.
+  13-19:
+    destruct_scopes; econstructor; econstructor; auto; econstructor;
+    [apply match_pattern_list_tuple_vars|]; simpl; econstructor; auto; econstructor;
+    [apply match_pattern_list_tuple_vars|]; constructor; auto;
+    constructor; auto.
+  13-19:
+    destruct_scopes; econstructor; econstructor; auto; econstructor;
+    [apply match_pattern_list_map_vars|];
+    simpl; econstructor; auto; econstructor;
+    [apply match_pattern_list_map_vars|]; constructor; auto;
+    constructor; auto.
+  * epose proof (H [FCase1 [([PLit l], `ttrue, `VNil);([PVar], `ttrue , °inf)]] ltac:(scope_solver) _) as H0; repeat deriv.
+    - simpl in H9. destruct Lit_beq eqn:EQ.
+      + apply Lit_eqb_eq in EQ. subst. choose_compat_lemma.
+      + congruence.
+    - inv H8. cbn in H11. repeat deriv. now apply inf_diverges in H11.
+    - inv H8.
+  Unshelve.
+    econstructor; econstructor; auto; econstructor;
+    [simpl; rewrite Lit_eqb_refl; reflexivity|];
+    simpl; econstructor; auto; econstructor;
+    [simpl; rewrite Lit_eqb_refl; reflexivity|]; constructor; auto;
+    constructor; auto.
+  * choose_compat_lemma.
+    - apply IHv1. destruct_scopes. split. 2: split. 1-2: auto.
+      intros. epose proof (H (FCase1 [([PCons PVar PVar], `ttrue, `VVar 0);([PVar], `ttrue , °inf)] :: F) ltac:(scope_solver) _) as H2; repeat deriv.
+      + inv H16. cbn in H17. repeat deriv. inv H16. cbn in H17. now exists k1.
+      + inv H16.
+      + inv H15.
+    - apply IHv2. destruct_scopes. split. 2: split. 1-2: auto.
+      intros. epose proof (H (FCase1 [([PCons PVar PVar], `ttrue, `VVar 1);([PVar], `ttrue , °inf)] :: F) ltac:(scope_solver) _) as H2; repeat deriv.
+      + inv H16. cbn in H17. repeat deriv. inv H16. cbn in H17. now exists k1.
+      + inv H16.
+      + inv H15.
+  Unshelve.
+    all: auto.
+    all: destruct H1; destruct_scopes; econstructor; econstructor; auto;
+       econstructor; [reflexivity|]; simpl; econstructor; auto;
+       econstructor; [reflexivity|]; eauto.
+  * choose_compat_lemma.
+    revert l0 Hcl2 H. induction l; destruct l0; intros.
+    - now auto.
+    - epose proof (H [FCase1 [([PTuple  []], `ttrue, `VNil);([PVar], `ttrue , °inf)]] ltac:(scope_solver) _) as H0; repeat deriv.
+      + inv H9.
+      + cbn in H11. repeat deriv. now apply inf_diverges in H12.
+      + now inv H8.
+    - epose proof (H [FCase1 [([PTuple  (repeat PVar (length (a :: l)))], `ttrue, `VNil);([PVar], `ttrue , °inf)]] ltac:(scope_solver) _) as H0; repeat deriv.
+      + inv H9.
+      + cbn in H11. repeat deriv. now apply inf_diverges in H12.
+      + now inv H8.
+    - inv IHv.
+      (* assert (REDCLOSED (`VTuple l) /\ REDCLOSED (`VTuple l0)) as [IS1 IS2]. {
+        destruct_scopes. split; do 3 constructor; intros;
+        try apply (H4 (S i)); try apply (H5 (S i)); slia.
+      }
+      assert (forall F : FrameStack, FSCLOSED F -> | F, ` VTuple l | ↓ -> | F, ` VTuple l0 | ↓) as IS3. {
+        intros.
+        epose proof (H (FCase1 [([PTuple (repeat PVar (length (a :: l)))], `ttrue, `VTuple (varsFrom 1 (length l)));([PVar], `ttrue , °inf)] :: F)) as H4.
+
+      }
+      specialize (IHl H3 IS1 _ IS2 IS3).
+     *)
+      constructor; auto.
+      + clear IHl. apply H2. split. 2: split.
+        1-2: do 2 constructor; destruct_scopes; try apply (H4 0); try apply (H5 0); slia.
+        intros. epose proof (H [FCase1 [([PTuple (repeat PVar (length (a :: l)))], `ttrue, `VVar 0);([PVar], `ttrue , °inf)]] ltac:(scope_solver) _) as H4; repeat deriv.
+        ** pose proof (match_pattern_list_tuple_vars (v :: l0)) as H1.
+           simpl repeat in H1. rewrite H1 in H14.
+      + apply IHl.
 Qed.
 
 Lemma Erel_Val_compat_reverse :
